SubroutineShare.v
@@ -1,27 +1,42 @@
 Require Import List.
 Import ListNotations.
 Require Import Bool.
-Require Import Coq.Logic.FunctionalExtensionality.
-Require Import Omega.
+Require Import Nat.
 Require Import Trace.
 Require Import Machine.
 Require Import ObsTrace.
+Require Import TraceProperties.
 
+(* To introduce sharing, we extend our domain model with two new domains:
+   Passed indicates memory that is sealed by a function but explicitly designated
+   to allow the immediate callee to access it. Shared indicates memory that has been
+   explicitly exempted from the sealing convention; once shared, it cannot be sealed
+   until the function activation that sealed it has returned.
+
+   Unlike sealing, sharing and passing require compiler input to identify instructions
+   that share or pass a location. A typical passing instruction is a write to the end
+   of the caller's frame, which will be read as a passed argument by the callee. The
+   canonical example of sharing is taking the address of a stack variable without
+   proving that the address will not escape. There is then no longer a guarantee that
+   it will remain protected.
+
+   Some systems make further guarantees, such as using capabilities to ensure that if
+   a pointer escapes, the object in question is only accessed in a memory safe way.
+   We regard this as a separate property that might well be enforced in parallel to
+   stack safety, but is outside of its scope.
+ *)
 Section DOMAIN_MODEL.
-
-  Inductive ShareStatus :=
-  | Local
-  | Passed
-  | Shared.
   
   Inductive StackDomain :=
-  | Claimed (d:nat)
-  | Unclaimed
+  | Sealed (d:nat)
+  | Shared (d:nat)
+  | Passed (d:nat)
+  | Unsealed
   | Outside
   .
 
   (* All components belong to domain, and a domain map tells us which. *)
-  Definition DomainMap := Component -> (StackDomain * ShareStatus).
+  Definition DomainMap := Component -> StackDomain.
   
 End DOMAIN_MODEL.
 
@@ -31,31 +46,24 @@ Section WITH_MAPS.
   Variable sm : Addr -> bool. (* Determines whether an address is in the stack. *)
   Variable pOf : MachineState -> PolicyState. (* Policy initialization function. *)
 
-  (* We will use the machinery defined at the end of Machine.v to extend traces of the
-     machine with context that will inform our properties. In this case the context is a
-     pair of a Domain Map and a natural number representing the depth of the stack. *)
-
+  Definition SealingConvention : Type := MachineState -> Addr -> bool.
+  Variable sc : SealingConvention.
+  
   Definition context : Type := DomainMap * nat.
 
-  (* For the initial context, we construct a domain map that maps the stack to Accessible
+  (* For the initial context, we construct a domain map that maps the stack to Unsealed
      and everything else to Outside. The stack depth is 0. *)
   Definition initC : context :=
     let dm := fun k =>
                 match k with
                 | Mem a =>
                   if sm a
-                  then (Unclaimed,Local)
-                  else (Outside,Shared)
-                | _ => (Outside,Shared)
+                  then Unsealed
+                  else Outside
+                | _ => Outside
                 end in
     (dm, O).
   
-  (* Our update function checks an "annotation" on the code being executed.
-     Annotations are defined in Machine.v as an alternative to a million different
-     maps, and the ones that matter here are call and return.
-
-     Annotations are given by the compiler. We assume that the compiler can tell us
-     which instructions represent calls and returns. *)
   Definition updateC (m:MachineState) (prev:context) : context :=
     let '(dm, d) := prev in
     match AnnotationOf cdm (m (Reg PC)) with
@@ -64,31 +72,40 @@ Section WITH_MAPS.
                    match k with
                    | Mem a =>
                      match f m a, dm k with
-                     | Some true, (Unclaimed,Local) => (Unclaimed,Passed)
-                     | Some false, (Unclaimed,_) => (Unclaimed,Shared)
+                     | Some true, Unsealed => Passed d
+                     | Some false, Unsealed => Shared d
                      | _, _ => dm k
                      end
                    | _ => dm k
                    end in
       (dm', d)
-    | Some call => (* A call adjusts the domain map by marking the caller's frame "inactive" *)
-                   (* and wrapping the remaining stack in a new instance of "active" *)
+    | Some call =>
       let dm' := fun k =>
-                    match k, dm k with
-                    | _, (Outside,ss) => (Outside,ss)
-                    | Mem a, (Unclaimed,ss) =>
-                      if wlt a (m (Reg SP))
-                      then (Claimed d,ss)
-                      else (Unclaimed,Local)
+                    match k, dm k with                      
+                    | _, Sealed d => Sealed d
+                    | _, Outside => Outside
+                    | Mem a, _ =>
+                      if sc m a
+                      then Sealed d
+                      else Unsealed (* If addresses are marked to be shared but the sealing convention
+                                       wants them unsealed, the sealing convention takes precedence *)
                     | _, _ => dm k
                     end in
       (dm', d+1)
-    | Some ret => (* A return unwraps the outermost domain of all components in the initial stack *)
+    | Some ret => 
       let dm' := fun k =>
                     match dm k with
-                    | (Claimed d', ss) =>
-                      if d =? d'
-                      then (Unclaimed,Local)
+                    | Sealed d' =>
+                      if (d-1) =? d' (* Sealed addresses are unsealed when their sealer is returned to. *)
+                      then Unsealed
+                      else dm k
+                    | Passed d' =>
+                      if (d-1) =? d' (* The same is true of passed addresses; they are single-use *)
+                      then Unsealed
+                      else dm k
+                    | Shared d' =>
+                      if d =? d' (* But shared addresses persist until the sharer itself returns *)
+                      then Unsealed
                       else dm k
                     | _ => dm k
                     end in
@@ -96,231 +113,93 @@ Section WITH_MAPS.
     | _ => (dm, d)
     end.
 
-  (* A component is inaccessible if it is claimed and local, or claimed by a
-     depth that is buried in the stack. *)
+  (* A component is inaccessible for writes if it is sealed or if it is passed by the a
+     function other than the current one, or its immediate caller. *)
   Definition Inaccessible (c:context) (k:Component) : Prop :=
     exists d,
-      fst c k = (Claimed d, Local) \/
-      (fst c k = (Claimed d, Passed) /\ d < (snd c)-1).
-  
-  (* Now it's quite simple to define an "ultra eager" integrity property:
-     if we run from any initial state, updating the context as above, then
-     at any particular state where a component k is in an Inaccessible domain,
-     k has the same value in the following state (if any.) We term this property
-     ultra eager because it "checks" at each step that components that are inaccessible
-     don't change, the most frequent it is possible to check. *)
-  Definition SimpleStackIntegrityUE : Prop :=
-    forall minit MCP k mcp mcp',
-      WithContextMP updateC initC (MPTraceOf (minit, pOf minit)) MCP ->
-      ContextSegment (fun _ _ => False) MCP (notfinished mcp (finished mcp')) ->
+      fst c k = (Sealed d) \/
+      (fst c k = (Passed d) /\ d < (snd c)-1).
+
+  (* So we can do ultra eager integrity, like before. *)
+  Definition StackIntegrityUE : Prop :=
+    forall minit k mcp mcp',
+      FindSegmentMP updateC (fun _ _ => False) (minit, pOf minit) initC (notfinished mcp (finished mcp')) ->
       Inaccessible (cstate mcp) k ->
       mstate mcp k = mstate mcp' k.
 
-    (* We can do a similar ultra eager style property with confidentiality, and since we're
-       not allowing sharing it is straightforward. But some preliminaries on confidentiality.
-       Firstly: confidentiality is expressed in terms of "variant" states. A K-variant
-       state of m is a state that agrees with m at every component not in the set K. It may also
-       agree at some components in K. The intuition is that if the step from a state changes the
-       state in the same way as the step from its K-variant, we can't tell from that step what
-       value a component in K was, so K is secret. *)
-  Definition variantOf (K : Component -> Prop) (m n : MachineState) :=
-    forall k, ~ K k -> m k = n k.
-  
-  (* "Changing the state in the same way" means that any component that changed is
-     one trace ends with the same value in the other. *)
-  Definition sameDifference (m m' n n' : MachineState) :=
-    forall k,
-      (m k <> m' k \/ n k <> n' k) ->
-      m' k = n' k.
-
-  (* Once again, we take adjacent pairs of states in the trace from an arbitrary
-     start state and check that a property holds between them. In this case, that
-     in any K-variant of the first state where K is the set of components that are
-     Inacessible in that state, the step has the same observable behavior and makes
-     the same changes to state. *)
-  Definition SimpleStackConfidentialityUE : Prop :=
-    forall minit MCP m dm d p m' dm' d' p' n o n' p'' o',
-      WithContextMP updateC initC (MPTraceOf (minit, pOf minit)) MCP ->
-      ContextSegment (fun _ _ => False) MCP (notfinished (m,(dm,d),p) (finished (m',(dm',d'),p'))) ->
-      variantOf (fun k => Inaccessible (dm,d) k) m n ->
-      mpstep (m,p) = Some (m',p',o) ->
-      mpstep (n,p) = Some (n',p'',o') ->
-      sameDifference m m' n n' /\ p = p'' /\ o = o'.
-
-  (* Once again, because this doesn't track initialization,
-     it doesn't actually fully work for the unclaimed memory. *)
-
-  (* Here are some helper relations to combine the addition of context to a trace,
-     and the segmenting of the resulting trace by a proposition P.*)
-  Definition FindSegmentMP P mp c MCP :=
-    exists MCP',
-      WithContextMP updateC c (MPTraceOf mp) MCP' /\
-      ContextSegment P MCP' MCP.
-
-  Definition FindSegmentM P m c MC :=
-    exists MC',
-      WithContextM updateC c (MTraceOf m) MC' /\
-      ContextSegmentM P MC' MC.
-
-  (* For integrity, ultra eager properties are significantly stronger than we actually
-     need. In fact, we want to consider lazy policies that allow illegal writes at times
-     in the name of efficiency. So we should consider what our actual goal is here - what
-     use are these properties? Here is an example of how we might think of a program logic
-     call rule that lets us guarantee that from a call point, if execution returns to the
-     caller, Inaccessible components are preserved. *)
-  
+  (* The call rule equivalent is identical except for similar changes in scope. *)
   Definition CallRule : Prop :=
-    forall minit MCP mcall dmcall dcall pcall,
+    forall minit MCP mcall dmcall dcall pcall mp o m' c' p' MCP',
       WithContextMP updateC initC (MPTraceOf (minit, pOf minit)) MCP ->
       InTrace (mcall,(dmcall,dcall),pcall) MCP ->
       AnnotationOf cdm (mcall (Reg PC)) = Some call ->
-         (* Case 1: Divergence (including due to failstop) *)
-      (forall MCP' m' dm d p',
-          WithContextMP updateC (dmcall,dcall) (MPTraceOf (mcall,pcall)) MCP' ->
-          InTrace (m',(dm,d),p') MCP' ->
-          d > dcall)
-      \/ (* Case 2: Return *)
-      (exists mp o m' c' p' MCP',
-          mpstep (mcall,pcall) = Some (mp,o) /\
-          FindSegmentMP (fun m '(dm,d) => d > dcall) mp (updateC mcall (dmcall,dcall)) MCP' /\
-          Last MCP' (m',c',p') /\
-          forall a,
-            wlt a (mcall (Reg SP)) = true ->
-            mcall (Mem a) = m' (Mem a)).
+      mpstep (mcall,pcall) = Some (mp,o) ->
+      FindSegmentMP updateC (fun m '(dm,d) => d > dcall) mp (updateC mcall (dmcall,dcall)) MCP' ->
+      Last MCP' (m',c',p') ->
+      justRet (ms mp) m' /\
+      forall a,
+        sc mcall a = true ->
+        mcall (Mem a) = m' (Mem a).      
 
-  (* We could use this as our ultimate specification, or just to guide our trace
-     properties. Note that this rule cares nothing for what happens to the state of
-     the Inaccessible components during the call, only that whe we return, they are
-     the same. Our eager property reflects this; instead of guaranteeing that they never
-     change, it guarantees that they are unchanged if and when the function returns. *)
-  
-  Definition SimpleStackIntegrityEager : Prop :=
-    forall minit MCP d k mcp mcp',
-      FindSegmentMP  (fun m c => snd c = d) (minit, pOf minit) initC MCP ->
-      mcp = head MCP ->
-      Inaccessible (cstate mcp) k ->
-      Last MCP mcp' ->
-      mstate mcp k = mstate mcp' k.
+  (* We can use our nice trace properties (redefined in TraceProperties.v to handle different
+     context types) to implement the integrity property. *)
+  Definition StackIntegrityEager : Prop :=
+    forall minit MCP d,
+      FindSegmentMP updateC (fun m c => snd c = d) (minit, pOf minit) initC MCP ->
+      TraceIntegrityEager (Inaccessible (cstate (head MCP))) MCP.
 
+  (* And it ought to imply the call rule. *)
   Theorem EagerIntSufficient :
-    SimpleStackIntegrityEager ->
+    StackIntegrityEager ->
     CallRule.
   Proof.
   Admitted.
   
-  (* We can make a similar argument about confidentiality, though it may be odd to
-     think of a confidentiality call rule. We can at least think of the following as
-     the "caller's view" of confidentiality: that from the call to the return, its
-     Inaccessible memory ought change nothing about the observable behavior of the
-     machine, and if control returns, its Inaccessible memory also did not impact the
-     returned state. *)
-
+  (* I won't rehash the ultra eager confidentiality here, but move on to the equivalent
+     confidentiality rule. We now allow reading of shared memory, and passed by the
+     appropriate function. *)
   Definition ConfRule : Prop :=
     forall minit MCP mcall dmcall dcall pcall n MCP' N MO NO,
       WithContextMP updateC initC (MPTraceOf (minit, pOf minit)) MCP ->
       InTrace (mcall,(dmcall,dcall),pcall) MCP ->
       AnnotationOf cdm (mcall (Reg PC)) = Some call ->
-      variantOf (fun k => Inaccessible (dmcall,dcall) k \/ fst (dmcall k) = Unclaimed) mcall n ->
+      variantOf (fun k => dmcall k = Unsealed \/ Inaccessible (dmcall,dcall) k) mcall n ->
       (* Clause 1: output up to return identical *)
       PrefixUpTo (fun '(_,(dm,d),_) => d = dcall) MCP MCP' ->
-      FindSegmentM (fun _ '(dm,d) => d = dcall) n (dmcall,dcall) N ->
+      FindSegmentMP updateC (fun _ '(dm,d) => d = dcall) (n,pcall) (dmcall,dcall) N ->
       ObsOfMCP MCP' MO ->
-      ObsOfMC N NO ->
-      ObsOfMP MO ~=_O ObsOfM NO /\
+      ObsOfMCP N NO ->
+      ObsOfMP MO ~=_O ObsOfMP NO /\
       (* Clause 2: if return, then state changes the same *)
       (forall m' dm' p',
           Last MCP' (m',(dm',dcall),p') ->
           exists n' dm'',
-            Last N (n',(dm'',dcall)) /\
+            Last N (n',(dm'',dcall),p') /\
             sameDifference mcall m' n n').
 
-  (* The flip side of the caller's rule is the trace property that holds on subtraces
-     representing calls. This only needs to be strong enough to support the caller-side
-     reasoning, so here is an example of such an eager (but not ultra-eager) property. *)
-  Definition SimpleStackConfidentialityEager : Prop :=
-    forall minit M MO d m dm p n N NO,
+  Definition StackConfidentialityEager : Prop :=
+    forall minit MCP d m dm p,
       let P := (fun m c => snd c = d) in
-      FindSegmentMP P (minit, pOf minit) initC M ->
-      head M = (m,(dm,d),p) ->
-      variantOf (fun k => Inaccessible (dm,d) k \/ fst (dm k) = Unclaimed) m n ->
-      FindSegmentM P n (dm,d) N ->
-      ObsOfMCP M MO ->
-      ObsOfMC N NO ->
-         (* Case 1 *)
-      (forall mend dmend pend,
-          Last M (mend,dmend,pend) ->
-          ~ P mend (dm,d) ->
-          exists nend dnend,
-            Last N (nend,dnend) /\
-            ObsOfMP MO ~=_O ObsOfM NO /\
-            sameDifference m mend n nend)
-      /\ (* Case 2 *)
-      (Infinite M ->
-       ObsOfMP MO ~=_O ObsOfM NO)
-      /\ (* Case 3 *)
-      (forall mend dmend pend,
-          Last M (mend, dmend, pend) ->
-          P mend (dm,d) ->
-          ObsOfMP MO <=_O ObsOfM NO).
+      let K := (fun k => Inaccessible (dm,d) k \/ dm k = Unsealed) in
+      FindSegmentMP updateC P (minit, pOf minit) initC MCP ->
+      head MCP = (m,(dm,d),p) ->
+      TraceConfidentialityEager updateC K P MCP.
 
   Theorem EagerConfSufficient :
-    SimpleStackConfidentialityEager ->
+    StackConfidentialityEager ->
     ConfRule.
   Proof.
   Admitted.
 
-  (* Now the above properties do a few things all at once that it helps to disentangle. They
-     quantify over all initial states, then over all segments of a trace at or above a certain
-     depth on the stack, ending with the return when the depth is reduced. And they state
-     properties of those segments. Lets focus on just capturing what it means for a trace
-     to respect the integrity and confidentiality of components, and separate out the finding
-     of the traces. The predicate K will indicate the set of components that must be protected. *)
-
-  Definition TraceIntegrityEager (K : Component -> Prop) (MCP:MCPTrace) : Prop :=
-    forall k (mcp':@MCPState context),
-      K k->
-      Last MCP mcp' ->
-      mstate (head MCP) k = mstate mcp' k.
-
-  (* The confidentiality trace property needs to know when the variant trace can be considered to have
-     returned, for which it takes a predicate on states and contexts, P. *)
-  Definition TraceConfidentialityEager (K : Component -> Prop)
-             (P:MachineState -> context -> Prop)
-             (MCP:@MCPTrace context) : Prop :=
-    forall MCP MO d m dm p n N NO,
-      head MCP = (m,(dm,d),p) ->
-      variantOf K m n ->
-      FindSegmentM P n (dm,d) N ->
-      ObsOfMCP MCP MO ->
-      ObsOfMC N NO ->
-         (* Case 1 *)
-      (forall mend dmend pend,
-          Last MCP (mend,dmend,pend) ->
-          ~ P mend (dm,d) ->
-          exists nend dnend,
-            Last N (nend,dnend) /\
-            ObsOfMP MO ~=_O ObsOfM NO /\
-            sameDifference m mend n nend)
-      /\ (* Case 2 *)
-      (Infinite MCP ->
-       ObsOfMP MO ~=_O ObsOfM NO)
-      /\ (* Case 3 *)
-      (forall mend dmend pend,
-          Last MCP (mend, dmend, pend) ->
-          P mend (dm,d) ->
-          ObsOfMP MO <=_O ObsOfM NO).
-
-  (* Now we can quantify over all initial states and segments starting with calls,
-     to create a property of the system that all calls enjoy both confidentiality and
-     integrity. *)
   Definition StackSafety :=
     forall minit MCP m dm d p,
       let P := (fun m '(dm, d') => d' >= d) in
-      FindSegmentMP P (minit, pOf minit) initC MCP ->
+      FindSegmentMP updateC P (minit, pOf minit) initC MCP ->
       head MCP = (m,(dm,d),p) ->
-      let K := (fun k => Inaccessible (dm,d) k) in
-      TraceIntegrityEager K MCP /\
-      TraceConfidentialityEager K P MCP.
+      let Ki := (fun k => Inaccessible (dm,d) k) in
+      TraceIntegrityEager Ki MCP /\
+      let Kc := (fun k => Inaccessible (dm,d) k) in
+      TraceConfidentialityEager updateC Kc P MCP.
 
   Theorem StackSafetySufficient :
     StackSafety ->
@@ -328,47 +207,6 @@ Section WITH_MAPS.
   Proof.
   Admitted.
 
-  (* ***** Control Flow Properties ***** *)
-  (* The addition of sharing does not change these. *)
+  (* Continued and (for now) concluded in Coroutine.v *)
   
-  Definition ControlSeparation : Prop :=
-    forall minit m1 p1 m2 p2 o f1 f2 ann1 ann2,
-      InTrace (m1,p1) (MPTraceOf (minit, pOf minit)) ->
-      mpstep (m1,p1) = Some (m2, p2,o) ->
-      cdm (m1 (Reg PC)) = inFun f1 ann1 ->
-      cdm (m2 (Reg PC)) = inFun f2 ann2 ->
-      f1 <> f2 ->
-      AnnotationOf cdm (m1 (Reg PC)) = Some call \/
-      AnnotationOf cdm (m1 (Reg PC)) = Some ret \/
-      AnnotationOf cdm (m1 (Reg PC)) = Some yield.
-
-  Definition YieldBackIntegrity : Prop :=
-    forall mp mp1 mp2 MPout,
-      InTrace mp1 (MPTraceOf mp) ->
-      AnnotationOf cdm (ms mp1 (Reg PC)) = Some yield ->
-      SplitInclusive (fun mp2 => sm (ms mp1 (Reg PC)) = sm (ms mp (Reg PC))) (MPTraceOf mp) MPout (MPTraceOf mp2) ->
-      justRet (ms mp1) (ms mp2).
-
-  Definition ReturnIntegrity : Prop :=
-    forall d minit MCP m c p m' c' p',
-      FindSegmentMP (fun m '(dm,d') => d' >= d) (minit, pOf minit) initC MCP ->
-      head MCP = (m,c,p) ->
-      Last MCP (m',c',p') ->
-      justRet m m'.
-
-  Variable em:EntryMap.
-  
-  Definition EntryIntegrity : Prop :=
-  forall minit mp1 m2 p2 o,
-    InTrace mp1 (MPTraceOf (minit, pOf minit)) ->
-    mpstep mp1 = Some (m2,p2,o) ->
-    AnnotationOf cdm (ms mp1 (Reg PC)) = Some call ->
-    em (m2 (Reg PC)).
-
-  Definition WellBracketedControlFlow  : Prop :=
-    ControlSeparation /\
-    ReturnIntegrity /\
-    YieldBackIntegrity /\
-    EntryIntegrity.
-
 End WITH_MAPS.
